cases.v
@@ -19,3 +19,20 @@ Proof.
       (intros; apply constructive_indefinite_description; ycrush).
   yelles 2.
 Qed.
+
+Inductive par_clos_cases (R : relation term) : term -> term -> Set :=
+| par_clos_cases_base : forall x y, R x y -> par_clos_cases R x y
+| par_clos_cases_bot : par_clos_cases R bot bot
+| par_clos_cases_var : forall n, par_clos_cases R (var n) (var n)
+| par_clos_cases_app : forall x y x' y', par_clos R x x' -> par_clos R y y' ->
+                                         par_clos_cases R (app x y) (app x' y')
+| par_clos_cases_abs : forall x y, par_clos R x y -> par_clos_cases R (abs x) (abs y).
+
+Lemma lem_par_clos_cases {R : relation term} : forall t s, par_clos R t s -> par_clos_cases R t s.
+Proof.
+  enough (H: forall t s, par_clos R t s -> { p : par_clos_cases R t s | True }) by
+      (intros t s H0; generalize (H t s H0); ycrush).
+  enough (forall t s, par_clos R t s -> exists p : par_clos_cases R t s, True) by
+      (intros; apply constructive_indefinite_description; ycrush).
+  yelles 2.
+Qed.
