sim.v
@@ -1,0 +1,324 @@
+Require Import beta.
+Require Import cases.
+
+Section Sim.
+
+Variable U : term -> Prop.
+
+Lemma lem_U_morphism : meaningless U -> forall x y, U x -> x == y -> U y.
+Proof.
+  intros.
+  assert (inf_beta x y) by (pose_inf_beta; ycrush).
+  sauto.
+Qed.
+
+Lemma lem_sim_morphism : meaningless U -> morphism (sim U).
+Proof.
+  intro Hm.
+  unfold morphism.
+  coinduction CH.
+  - clear CH; pose lem_U_morphism; ycrush.
+  - destruct x'0, y'0; try solve [ clear CH; sauto ].
+    intros.
+    apply par_clos_app.
+    + apply CH with (x := x0) (y := x'); clear CH; pose_term_eq; ycrush.
+    + apply CH with (x := y0) (y := y'); clear CH; pose_term_eq; ycrush.
+Qed.
+
+Lemma lem_par_bot_to_sim :
+  U bot -> forall x y, par_bot U x y -> sim U x y.
+Proof.
+  intro; coinduction using ssolve.
+Qed.
+
+Lemma lem_sim_refl_0 : reflexive term (sim U).
+Proof.
+  coinduction on 0.
+Qed.
+
+Lemma lem_sim_refl :
+  (forall x y, U x -> x == y -> U y) -> forall x y, x == y -> sim U x y.
+Proof.
+  intro; coinduction.
+Qed.
+
+Lemma lem_sim_sym : symmetric term (sim U).
+Proof.
+  coinduction.
+Qed.
+
+Lemma lem_sim_trans : meaningless U -> transitive term (sim U).
+Proof.
+  unfold meaningless.
+  intro H; simp_hyps.
+  coinduction CH using auto.
+  - csolve CH.
+  - cintro; [ pose lem_sim_sym; clear CH; constructor; sintuition; eauto |
+              constructor 4; eapply CH; eauto ].
+  - cintro; [ pose lem_sim_sym; clear CH; constructor; sintuition; eauto |
+              constructor 5; eapply CH; eauto ].
+Qed.
+
+Lemma lem_sim_shift_closed : meaningless U -> shift_closed (sim U).
+Proof.
+  unfold shift_closed.
+  intro H.
+  coinduction.
+Qed.
+
+Lemma lem_sim_subst : meaningless U ->
+                      forall n t t' s s', sim U t t' -> sim U s s' -> sim U (t [n := s]) (t' [n := s']).
+Proof.
+  intro H.
+  pose lem_sim_shift_closed; coinduction.
+Qed.
+
+CoFixpoint F_sim_to_par_bot (t s : term) (p : sim U t s) : term.
+destruct (lem_par_clos_cases t s p).
+- exact bot.
+- exact bot.
+- exact (var n).
+- exact (app (F_sim_to_par_bot x x' p0) (F_sim_to_par_bot y y' p1)).
+- exact (abs (F_sim_to_par_bot x y p0)).
+Defined.
+
+Lemma lem_sim_to_par_bot : forall t s, sim U t s -> exists r, par_bot U t r /\ par_bot U s r.
+Proof.
+  enough (exists f, forall t s (p : sim U t s), par_bot U t (f t s p) /\ par_bot U s (f t s p)) by ycrush.
+  exists F_sim_to_par_bot.
+  split; revert t s p.
+  - cofix CH.
+    intros t s p.
+    peek (F_sim_to_par_bot t s p).
+    destruct (lem_par_clos_cases t s p).
+    + clear CH; destruct x; sauto; constructor; constructor; pose_term_eq; ycrush.
+    + clear CH; solve [ constructor ].
+    + clear CH; solve [ constructor ].
+    + apply par_clos_app; apply CH.
+    + apply par_clos_abs; apply CH.
+  - cofix CH.
+    intros t s p.
+    peek (F_sim_to_par_bot t s p).
+    destruct (lem_par_clos_cases t s p).
+    + clear CH; destruct y; sauto; constructor; constructor; pose_term_eq; ycrush.
+    + clear CH; solve [ constructor ].
+    + clear CH; solve [ constructor ].
+    + apply par_clos_app; apply CH.
+    + apply par_clos_abs; apply CH.
+Qed.
+
+Lemma lem_step_beta_preserves_sim : meaningless U ->
+  forall t t' s, step_beta t s -> sim U t t' -> exists s', step_beta_eq t' s' /\ sim U s s'.
+Proof.
+  intros Hm t t' s H; revert t'.
+  induction H.
+  - inversion_clear H.
+    intros t' H.
+    inversion H; subst; clear H; try yelles 1.
+    + exists t'; split.
+      * pose_term_eq; ycrush.
+      * assert (inf_beta x y) by
+            (rewrite H0; rewrite H1; pose lem_red_beta_redex; pose_inf_beta; ycrush).
+        ycrush.
+    + inversion H0; subst; yisolve; fold term_eq in *.
+      inversion H2; subst; try yelles 1.
+      * assert (U (abs t1)) by (pose lem_U_morphism; pose_term_eq; ycrush).
+        assert (U (app (abs t1) t2)) by ycrush.
+        exists (app x' y'); split.
+        ** pose_term_eq; ycrush.
+        ** assert (sim U (app x0 y0) (app x' y')) by ycrush.
+           assert (sim U (app (abs t1) t2) (app x' y')) by
+               (pose lem_sim_morphism; pose_term_eq; ycrush).
+           assert (inf_beta (app (abs t1) t2) y) by
+            (rewrite H1; pose lem_red_beta_redex; pose_inf_beta; ycrush).
+           ycrush.
+      * inversion H6; subst; yisolve; fold term_eq in *.
+        exists (y1 [0 := y']).
+        split.
+        ** pose lem_step_beta_redex; ycrush.
+        ** assert (sim U (x [0 := y0]) (y1 [0 := y'])) by
+              (pose lem_sim_subst; ycrush).
+           assert (y == x [0 := y0]) by
+               (rewrite H7; rewrite H8; assumption).
+           pose lem_sim_morphism; pose_term_eq; ycrush.
+  - intros t' H1.
+    inversion H1; subst.
+    + exists t'; split.
+      * pose_term_eq; ycrush.
+      * assert (inf_beta (app x y) (app x' y')) by
+            (rewrite H0; pose lem_red_beta_redex; pose_inf_beta; ycrush).
+        ycrush.
+    + generalize (IHcomp_clos x'0 H4); intro HH; destruct HH as [s' [HH1 HH2]].
+      exists (app s' y'0).
+      split.
+      * destruct HH1.
+        ** left; constructor 2; ycrush.
+        ** right; pose_term_eq; ycrush.
+      * constructor 4; pose lem_sim_morphism; pose_term_eq; unfold morphism, sim in *; ycrush.
+  - intros t' H1.
+    inversion H1; subst.
+    + exists t'; split.
+      * pose_term_eq; ycrush.
+      * assert (inf_beta (app x y) (app x' y')) by
+            (rewrite H0; pose lem_red_beta_redex; pose_inf_beta; ycrush).
+        ycrush.
+    + generalize (IHcomp_clos y'0 H6); intro HH; destruct HH as [s' [HH1 HH2]].
+      exists (app x'0 s').
+      split.
+      * destruct HH1.
+        ** left; constructor 3; ycrush.
+        ** right; pose_term_eq; ycrush.
+      * constructor 4; pose lem_sim_morphism; pose_term_eq; unfold morphism, sim in *; ycrush.
+  - intros t' H1.
+    inversion H1; subst.
+    + exists t'; split.
+      * pose_term_eq; ycrush.
+      * assert (inf_beta (abs x) (abs y)) by
+            (pose lem_red_beta_redex; pose_inf_beta; ycrush).
+        ycrush.
+    + generalize (IHcomp_clos y0 H2); intro HH; destruct HH as [s' [HH1 HH2]].
+      exists (abs s').
+      split.
+      * destruct HH1.
+        ** left; constructor 4; ycrush.
+        ** right; pose_term_eq; ycrush.
+      * constructor 5; pose lem_sim_morphism; pose_term_eq; unfold morphism, sim in *; ycrush.
+Qed.
+
+Lemma lem_red_beta_preserves_sim : meaningless U ->
+  forall t t' s, red_beta t s -> sim U t t' -> exists s', red_beta t' s' /\ sim U s s'.
+Proof.
+  intros Hm t t' s H; revert t'.
+  induction H.
+  - pose lem_sim_morphism; pose_term_eq; ycrush.
+  - intros.
+    generalize (lem_step_beta_preserves_sim Hm x t' y H H1); intro HH; destruct HH as [s [HH1 HH2]].
+    generalize (IHstar s HH2); intro Hs; destruct Hs as [s0 [Hs1 Hs2]].
+    exists s0.
+    destruct HH1; pose_red_beta; pose_term_eq; ycrush.
+Qed.
+
+Lemma lem_red_beta_preserves_sim_choice :
+  meaningless U ->
+  forall t t' s, red_beta t s -> sim U t t' -> { s' | red_beta t' s' /\ sim U s s' }.
+Proof.
+  intros.
+  apply constructive_indefinite_description.
+  eapply lem_red_beta_preserves_sim; eauto.
+Qed.
+
+Lemma lem_inf_beta_preserves_sim_cases :
+  meaningless U ->
+  forall t t' s, inf_beta t s -> sim U t t' ->
+                 red_beta t s \/
+                 (exists u, red_beta t' u /\ sim U s u) \/
+                 (exists s1 s2 t1 t2 u1 u2, s = app s1 s2 /\ red_beta t (app t1 t2) /\
+                                            inf_beta t1 s1 /\ inf_beta t2 s2 /\
+                                            sim U t1 u1 /\ sim U t2 u2 /\ red_beta t' (app u1 u2)) \/
+                 (exists s0 t0 u0, s = abs s0 /\ red_beta t (abs t0) /\ inf_beta t0 s0 /\
+                                   sim U t0 u0 /\ red_beta t' (abs u0)).
+Proof.
+  intros.
+  inversion H0; subst; yisolve.
+  - assert (HH: exists u, sim U (app x y) u /\ red_beta t' u) by
+        Reconstr.rcrush (@beta.lem_step_beta_to_red_beta, @beta.lem_red_beta_refl, @Sim.lem_red_beta_preserves_sim, @beta.lem_red_beta_step) (@beta.step_beta_eq).
+    destruct HH as [u [HH1 HH2]].
+    inversion HH1; subst.
+    + right; left.
+      exists u.
+      assert (inf_beta (app x y) (app x' y')) by
+          Reconstr.reasy (@beta.lem_inf_beta_app) (@defs.inf_beta, @defs.red_beta).
+      assert (U (app x' y')) by ycrush.
+      ycrush.
+    + right; right; left.
+      exists x', y', x, y, x'0, y'0.
+      ycrush.
+  - assert (HH: exists u, sim U (abs x) u /\ red_beta t' u) by
+        Reconstr.rcrush (@beta.lem_step_beta_to_red_beta, @beta.lem_red_beta_refl, @Sim.lem_red_beta_preserves_sim, @beta.lem_red_beta_step) (@beta.step_beta_eq).
+    destruct HH as [u [HH1 HH2]].
+    inversion HH1; subst.
+    + right; left.
+      exists u.
+      assert (inf_beta (abs x) (abs x')) by
+          Reconstr.reasy (@beta.lem_inf_beta_abs) (@defs.inf_beta, @defs.red_beta).
+      assert (U (abs x')) by ycrush.
+      ycrush.
+    + right; right; right.
+      exists x', x, y.
+      ycrush.
+Qed.
+
+Inductive ctr (t t' s : term) : Set :=
+| ctr_red : red_beta t s -> ctr t t' s
+| ctr_u : forall u, red_beta t' u -> sim U s u -> ctr t t' s
+| ctr_app : forall s1 s2 t1 t2 u1 u2, s = app s1 s2 -> red_beta t (app t1 t2) ->
+                                      inf_beta t1 s1 -> inf_beta t2 s2 ->
+                                      sim U t1 u1 -> sim U t2 u2 -> red_beta t' (app u1 u2) ->
+                                      ctr t t' s
+| ctr_abs : forall s0 t0 u0, s = abs s0 -> red_beta t (abs t0) -> inf_beta t0 s0 ->
+                             sim U t0 u0 -> red_beta t' (abs u0) -> ctr t t' s.
+
+Lemma lem_inf_beta_preserves_sim_cases_choice :
+  meaningless U ->
+  forall t t' s, inf_beta t s -> sim U t t' -> ctr t t' s.
+Proof.
+  intros Hm t t' s H1 H2.
+  enough ({ c : ctr t t' s | True }) by ycrush.
+  enough (exists c : ctr t t' s, True) by (apply constructive_indefinite_description; assumption).
+  generalize (lem_inf_beta_preserves_sim_cases Hm t t' s H1 H2).
+  ycrush.
+Qed.
+
+CoFixpoint F_inf_beta_preserves_sim (t t' s : term) (pu : meaningless U)
+           (p1 : inf_beta t s) (p2 : sim U t t') : term.
+destruct (lem_inf_beta_preserves_sim_cases_choice pu t t' s p1 p2).
+- exact (proj1_sig (lem_red_beta_preserves_sim_choice pu t t' s r p2)).
+- exact u.
+- exact (app (F_inf_beta_preserves_sim t1 u1 s1 pu i s0) (F_inf_beta_preserves_sim t2 u2 s2 pu i0 s3)).
+- exact (abs (F_inf_beta_preserves_sim t0 u0 s0 pu i s1)).
+Defined.
+
+Lemma lem_inf_beta_preserves_sim : meaningless U ->
+  forall t t' s, inf_beta t s -> sim U t t' -> exists s', inf_beta t' s' /\ sim U s s'.
+Proof.
+  intro Hm.
+  enough (exists f, forall t t' s (p1 : inf_beta t s) (p2 : sim U t t'),
+               inf_beta t' (f t t' s Hm p1 p2) /\ sim U s (f t t' s Hm p1 p2)) by ycrush.
+  exists F_inf_beta_preserves_sim.
+  split.
+  - revert t t' s p1 p2.
+    cofix CH.
+    intros.
+    peek (F_inf_beta_preserves_sim t t' s Hm p1 p2).
+    destruct (lem_inf_beta_preserves_sim_cases_choice Hm t t' s p1 p2).
+    + clear CH; destruct (lem_red_beta_preserves_sim_choice Hm t t' _ r p2); pose_inf_beta; ycrush.
+    + clear CH; pose_inf_beta; ycrush.
+    + apply inf_clos_app with (x := u1) (y := u2).
+      * assumption.
+      * apply CH.
+      * apply CH.
+    + apply inf_clos_abs with (x := u0).
+      * assumption.
+      * apply CH.
+  - revert t t' s p1 p2.
+    cofix CH.
+    intros.
+    peek (F_inf_beta_preserves_sim t t' s Hm p1 p2).
+    destruct (lem_inf_beta_preserves_sim_cases_choice Hm t t' s p1 p2).
+    + clear CH; destruct (lem_red_beta_preserves_sim_choice Hm t t' _ r p2); ycrush.
+    + clear CH; ycrush.
+    + rewrite e.
+      apply par_clos_app.
+      * apply CH.
+      * apply CH.
+    + rewrite e.
+      apply par_clos_abs.
+      apply CH.
+Qed.
+
+End Sim.
+
+Ltac pose_sim := pose proof lem_par_bot_to_sim; pose proof lem_sim_refl_0;
+                 pose proof lem_sim_refl; pose proof lem_sim_sym; pose proof lem_sim_trans;
+                 pose lem_sim_subst; pose lem_sim_to_par_bot;
+                 autounfold with shints in *.
