Makefile
@@ -1,4 +1,4 @@
-all : tactics.vo star.vo defs.vo equality.vo basics.vo beta.vo botred.vo cases.vo weak.vo crnf.vo root_active.vo nred.vo
+all : tactics.vo star.vo defs.vo equality.vo basics.vo beta.vo sim.vo botred.vo cases.vo weak.vo crnf.vo root_active.vo nred.vo
 
 tactics.vo : tactics.v
 	coqc tactics.v
@@ -6,7 +6,7 @@ tactics.vo : tactics.v
 defs.vo : defs.v
 	coqc defs.v
 
-cases.vo : cases.v defs.vo
+cases.vo : cases.v defs.vo tactics.vo
 	coqc cases.v
 
 equality.vo : equality.v defs.vo tactics.vo
@@ -21,19 +21,22 @@ basics.vo : basics.v equality.vo defs.vo tactics.vo star.vo equality.vo
 beta.vo : beta.v basics.vo
 	coqc beta.v
 
-botred.vo : botred.v beta.vo cases.vo
+sim.vo : sim.v beta.vo cases.vo
+	coqc sim.v
+
+botred.vo : botred.v beta.vo sim.vo cases.vo
 	coqc botred.v
 
 weak.vo : weak.v beta.vo
 	coqc weak.v
 
-crnf.vo : crnf.v beta.vo cases.vo
+crnf.vo : crnf.v weak.vo cases.vo
 	coqc crnf.v
 
-root_active.vo : root_active.v weak.vo
+root_active.vo : root_active.v weak.vo sim.vo
 	coqc root_active.v
 
-nred.vo : nred.v crnf.vo botred.vo
+nred.vo : nred.v crnf.vo botred.vo sim.vo
 	coqc nred.v
 
 clean:
